lib_list/ArrayListGen.fsti
@@ -62,13 +62,15 @@ val mem (#a:Type0) (x:nat) (hd:nat) (s:Seq.seq (cell a)) : prop
 /// at [hd]
 val ptrs_in (#a:Type) (hd:nat) (s:Seq.seq (cell a)) : GTot (FS.set nat)
 
-/// Set of all pointers contained in the three doubly linked lists
-let ptrs_all (#a:Type) (hd1 hd2 hd3:nat) (s:Seq.seq (cell a)) =
-  FS.union (ptrs_in hd1 s) (FS.union (ptrs_in hd2 s) (ptrs_in hd3 s))
+/// Set of all pointers contained in the four doubly linked lists
+let ptrs_all (#a:Type) (hd1 hd2 hd3 hd4:nat) (s:Seq.seq (cell a)) =
+  FS.union
+    (FS.union (ptrs_in hd1 s) (ptrs_in hd2 s))
+    (FS.union (ptrs_in hd3 s) (ptrs_in hd4 s))
 
 /// Membership of element [x] in any of the dlist pointed to by [hd1], [hd2], or [hd3]
-let mem_all (#a:Type0) (x:nat) (hd1 hd2 hd3:nat) (s:Seq.seq (cell a)) =
-  FS.mem x (ptrs_all hd1 hd2 hd3 s)
+let mem_all (#a:Type0) (x:nat) (hd1 hd2 hd3 hd4:nat) (s:Seq.seq (cell a)) =
+  FS.mem x (ptrs_all hd1 hd2 hd3 hd4 s)
 
 /// Equivalence lemma between `mem` and membership in `ptrs_in`
 val lemma_mem_ptrs_in (#a:Type)
@@ -95,13 +97,18 @@ val disjoint (#a:Type)
   (hd1 hd2: nat)
   : prop
 
-/// Mutual exclusiveness for three dlists
-let disjoint3 (#a:Type) (s:Seq.seq (cell a)) (hd1 hd2 hd3: nat) =
-  disjoint s hd1 hd2 /\ disjoint s hd1 hd3 /\ disjoint s hd2 hd3
+/// Mutual exclusiveness for four dlists
+let disjoint4 (#a:Type) (s:Seq.seq (cell a)) (hd1 hd2 hd3 hd4: nat) =
+  disjoint s hd1 hd2 /\
+  disjoint s hd1 hd3 /\
+  disjoint s hd1 hd4 /\
+  disjoint s hd2 hd3 /\
+  disjoint s hd2 hd4 /\
+  disjoint s hd3 hd4
 
-/// The array is partitioned exactly between the three lists
-let partition (#a:Type) (s:Seq.seq (cell a)) (hd1 hd2 hd3: nat) =
-  forall (i:nat{i < Seq.length s}). i == null \/ (FS.mem i (ptrs_all hd1 hd2 hd3 s))
+/// The array is partitioned exactly between the four lists
+let partition (#a:Type) (s:Seq.seq (cell a)) (hd1 hd2 hd3 hd4: nat) =
+  forall (i:nat{i < Seq.length s}). i == null \/ (FS.mem i (ptrs_all hd1 hd2 hd3 hd4 s))
 
 (** Some helpers to use cells *)
 
@@ -112,72 +119,93 @@ val write_data (#a:Type0) (c:cell a) (v:a) : cell a
 (** Steel functions and vprops *)
 
 /// The refinement predicate for varraylist, stating that the sequence contains
-/// three mutually exclusive doubly linked lists
+/// four mutually exclusive doubly linked lists
 let varraylist_refine (#a:Type)
-  (pred1 pred2 pred3: a -> prop)
-  (hd1 hd2 hd3:nat)
+  (pred1 pred2 pred3 pred4: a -> prop)
+  (hd1 hd2 hd3 hd4:nat)
   (s:Seq.seq (cell a)) : prop
-  = is_dlist pred1 hd1 s /\ is_dlist pred2 hd2 s /\ is_dlist pred3 hd3 s /\ disjoint3 s hd1 hd2 hd3
+  =
+  is_dlist pred1 hd1 s /\
+  is_dlist pred2 hd2 s /\
+  is_dlist pred3 hd3 s /\
+  is_dlist pred4 hd4 s /\
+  disjoint4 s hd1 hd2 hd3 hd4
 
 /// The main vprop of this module.
-/// We have access to an array, such that the array contains three mutually
+/// We have access to an array, such that the array contains four mutually
 /// exclusive doubly linked list, starting at offsets [hd1] [hd2] and [hd3]
 /// respectively
 [@@__steel_reduce__]
-let varraylist (#a:Type) (pred1 pred2 pred3: a -> prop) (r:A.array (cell a)) (hd1 hd2 hd3:nat) : vprop
-  = A.varray r `vrefine` (varraylist_refine pred1 pred2 pred3 hd1 hd2 hd3)
+let varraylist (#a:Type) (pred1 pred2 pred3 pred4: a -> prop) (r:A.array (cell a)) (hd1 hd2 hd3 hd4:nat) : vprop
+  = A.varray r `vrefine` (varraylist_refine pred1 pred2 pred3 pred4 hd1 hd2 hd3 hd4)
 
 /// Create an arraylist with an empty sequence
 val intro_arraylist_nil (#a:Type) (#opened:inames)
-  (pred1 pred2 pred3: a -> prop)
+  (pred1 pred2 pred3 pred4: a -> prop)
   (r:A.array (cell a))
-  (hd1 hd2 hd3:US.t) :
+  (hd1 hd2 hd3 hd4:US.t) :
   SteelGhost unit opened
     (A.varray r)
-    (fun _ -> varraylist pred1 pred2 pred3 r (US.v hd1) (US.v hd2) (US.v hd3))
+    (fun _ ->
+      varraylist pred1 pred2 pred3 pred4 r
+        (US.v hd1) (US.v hd2) (US.v hd3) (US.v hd4))
     (requires fun _ ->
       A.length r == 0 /\
       hd1 == null_ptr /\
       hd2 == null_ptr /\
-      hd3 == null_ptr)
+      hd3 == null_ptr /\
+      hd4 == null_ptr)
     (ensures fun _ _ h1 ->
-      h1 (varraylist pred1 pred2 pred3 r (US.v hd1) (US.v hd2) (US.v hd3)) `Seq.equal` Seq.empty
+      h1 (varraylist pred1 pred2 pred3 pred4 r
+        (US.v hd1) (US.v hd2) (US.v hd3) (US.v hd4))
+      `Seq.equal`
+      Seq.empty
     )
 
 /// If the head of one of the lists is not null, then it is in the list
 val lemma_head_not_null_mem (#a:Type) (#opened:inames)
-  (pred1 pred2 pred3: a -> prop)
+  (pred1 pred2 pred3 pred4: a -> prop)
   (r:A.array (cell a))
-  (hd1 hd2 hd3:US.t) :
+  (hd1 hd2 hd3 hd4:US.t) :
   SteelGhost unit opened
-    (varraylist pred1 pred2 pred3 r (US.v hd1) (US.v hd2) (US.v hd3))
-    (fun _ -> varraylist pred1 pred2 pred3 r (US.v hd1) (US.v hd2) (US.v hd3))
+    (varraylist pred1 pred2 pred3 pred4 r
+      (US.v hd1) (US.v hd2) (US.v hd3) (US.v hd4))
+    (fun _ ->
+      varraylist pred1 pred2 pred3 pred4 r
+        (US.v hd1) (US.v hd2) (US.v hd3) (US.v hd4))
     (requires fun _ -> True)
     (ensures fun h0 _ h1 ->
+      let gs0 = h0 (varraylist pred1 pred2 pred3 pred4 r
+        (US.v hd1) (US.v hd2) (US.v hd3) (US.v hd4)) in
+      let gs1 = h1 (varraylist pred1 pred2 pred3 pred4 r
+        (US.v hd1) (US.v hd2) (US.v hd3) (US.v hd4)) in
       // Framing
-      h0 (varraylist pred1 pred2 pred3 r (US.v hd1) (US.v hd2) (US.v hd3)) ==
-      h1 (varraylist pred1 pred2 pred3 r (US.v hd1) (US.v hd2) (US.v hd3)) /\
+      gs1 == gs0 /\
       // Functional property
-      (hd1 = null_ptr \/ mem (US.v hd1) (US.v hd1) (h1 (varraylist pred1 pred2 pred3 r (US.v hd1) (US.v hd2) (US.v hd3)))) /\
-      (hd2 = null_ptr \/ mem (US.v hd2) (US.v hd2) (h1 (varraylist pred1 pred2 pred3 r (US.v hd1) (US.v hd2) (US.v hd3)))) /\
-      (hd3 = null_ptr \/ mem (US.v hd3) (US.v hd3) (h1 (varraylist pred1 pred2 pred3 r (US.v hd1) (US.v hd2) (US.v hd3))))
+      (hd1 = null_ptr \/ mem (US.v hd1) (US.v hd1) gs1) /\
+      (hd2 = null_ptr \/ mem (US.v hd2) (US.v hd2) gs1) /\
+      (hd3 = null_ptr \/ mem (US.v hd3) (US.v hd3) gs1) /\
+      (hd4 = null_ptr \/ mem (US.v hd4) (US.v hd4) gs1)
     )
 
 /// If the head of one of the lists is not null, then it is smaller than the length
 /// of the underlying array
 val lemma_head1_in_bounds (#a:Type) (#opened:inames)
-  (pred1 pred2 pred3: a -> prop)
+  (pred1 pred2 pred3 pred4: a -> prop)
   (r:A.array (cell a))
   (hd1: US.t)
-  (hd2 hd3: Ghost.erased nat) :
+  (hd2 hd3 hd4: Ghost.erased nat) :
   SteelGhost unit opened
-    (varraylist pred1 pred2 pred3 r (US.v hd1) hd2 hd3)
-    (fun _ -> varraylist pred1 pred2 pred3 r (US.v hd1) hd2 hd3)
+    (varraylist pred1 pred2 pred3 pred4 r (US.v hd1) hd2 hd3 hd4)
+    (fun _ -> varraylist pred1 pred2 pred3 pred4 r (US.v hd1) hd2 hd3 hd4)
     (requires fun _ -> True)
     (ensures fun h0 _ h1 ->
+      let gs0 = h0 (varraylist pred1 pred2 pred3 pred4 r
+        (US.v hd1) hd2 hd3 hd4) in
+      let gs1 = h1 (varraylist pred1 pred2 pred3 pred4 r
+        (US.v hd1) hd2 hd3 hd4) in
       // Framing
-      h0 (varraylist pred1 pred2 pred3 r (US.v hd1) hd2 hd3) ==
-      h1 (varraylist pred1 pred2 pred3 r (US.v hd1) hd2 hd3) /\
+      gs1 == gs0 /\
       // Functional property
       (hd1 == null_ptr \/ US.v hd1 < A.length r)
     )
@@ -185,151 +213,171 @@ val lemma_head1_in_bounds (#a:Type) (#opened:inames)
 /// If the head of one of the lists is not null, then it is smaller than the length
 /// of the underlying array
 val lemma_head2_in_bounds (#a:Type) (#opened:inames)
-  (pred1 pred2 pred3: a -> prop)
+  (pred1 pred2 pred3 pred4: a -> prop)
   (r:A.array (cell a))
   (hd1: Ghost.erased nat)
   (hd2: US.t)
-  (hd3: Ghost.erased nat) :
+  (hd3 hd4: Ghost.erased nat) :
   SteelGhost unit opened
-    (varraylist pred1 pred2 pred3 r hd1 (US.v hd2) hd3)
-    (fun _ -> varraylist pred1 pred2 pred3 r hd1 (US.v hd2) hd3)
+    (varraylist pred1 pred2 pred3 pred4 r hd1 (US.v hd2) hd3 hd4)
+    (fun _ -> varraylist pred1 pred2 pred3 pred4 r hd1 (US.v hd2) hd3 hd4)
     (requires fun _ -> True)
     (ensures fun h0 _ h1 ->
+      let gs0 = h0 (varraylist pred1 pred2 pred3 pred4 r
+        hd1 (US.v hd2) hd3 hd4) in
+      let gs1 = h1 (varraylist pred1 pred2 pred3 pred4 r
+        hd1 (US.v hd2) hd3 hd4) in
       // Framing
-      h0 (varraylist pred1 pred2 pred3 r hd1 (US.v hd2) hd3) ==
-      h1 (varraylist pred1 pred2 pred3 r hd1 (US.v hd2) hd3) /\
+      gs1 == gs0 /\
       // Functional property
       (hd2 == null_ptr \/ US.v hd2 < A.length r)
     )
 
 /// If the head of one of the lists is not null, then it satisfies the corresponding predicate
 val lemma_head1_implies_pred1 (#a:Type) (#opened:inames)
-  (pred1 pred2 pred3: a -> prop)
+  (pred1 pred2 pred3 pred4: a -> prop)
   (r:A.array (cell a))
   (hd1:US.t{US.v hd1 < A.length r})
-  (hd2 hd3:US.t) :
+  (hd2 hd3 hd4:US.t) :
   SteelGhost unit opened
-    (varraylist pred1 pred2 pred3 r (US.v hd1) (US.v hd2) (US.v hd3))
-    (fun _ -> varraylist pred1 pred2 pred3 r (US.v hd1) (US.v hd2) (US.v hd3))
+    (varraylist pred1 pred2 pred3 pred4 r (US.v hd1) (US.v hd2) (US.v hd3) (US.v hd4))
+    (fun _ -> varraylist pred1 pred2 pred3 pred4 r (US.v hd1) (US.v hd2) (US.v hd3) (US.v hd4))
     (requires fun h -> hd1 <> null_ptr)
     (ensures fun h0 _ h1 ->
+      let gs0 = h0 (varraylist pred1 pred2 pred3 pred4 r
+        (US.v hd1) (US.v hd2) (US.v hd3) (US.v hd4)) in
+      let gs1 = h1 (varraylist pred1 pred2 pred3 pred4 r
+        (US.v hd1) (US.v hd2) (US.v hd3) (US.v hd4)) in
       // Framing
-      h0 (varraylist pred1 pred2 pred3 r (US.v hd1) (US.v hd2) (US.v hd3)) ==
-      h1 (varraylist pred1 pred2 pred3 r (US.v hd1) (US.v hd2) (US.v hd3)) /\
+      gs1 == gs0 /\
       // Functional property
-      pred1 (get_data (Seq.index (h1 (varraylist pred1 pred2 pred3 r (US.v hd1) (US.v hd2) (US.v hd3))) (US.v hd1)))
+      pred1 (get_data (Seq.index gs1 (US.v hd1)))
     )
 
 /// If the head of one of the lists is not null, then it satisfies the corresponding predicate
 val lemma_head2_implies_pred2 (#a:Type) (#opened:inames)
-  (pred1 pred2 pred3: a -> prop)
+  (pred1 pred2 pred3 pred4: a -> prop)
   (r:A.array (cell a))
   (hd1:US.t)
   (hd2:US.t{US.v hd2 < A.length r})
-  (hd3:US.t) :
+  (hd3 hd4:US.t) :
   SteelGhost unit opened
-    (varraylist pred1 pred2 pred3 r (US.v hd1) (US.v hd2) (US.v hd3))
-    (fun _ -> varraylist pred1 pred2 pred3 r (US.v hd1) (US.v hd2) (US.v hd3))
+    (varraylist pred1 pred2 pred3 pred4 r (US.v hd1) (US.v hd2) (US.v hd3) (US.v hd4))
+    (fun _ -> varraylist pred1 pred2 pred3 pred4 r (US.v hd1) (US.v hd2) (US.v hd3) (US.v hd4))
     (requires fun h -> hd2 <> null_ptr)
     (ensures fun h0 _ h1 ->
+      let gs0 = h0 (varraylist pred1 pred2 pred3 pred4 r
+        (US.v hd1) (US.v hd2) (US.v hd3) (US.v hd4)) in
+      let gs1 = h1 (varraylist pred1 pred2 pred3 pred4 r
+        (US.v hd1) (US.v hd2) (US.v hd3) (US.v hd4)) in
       // Framing
-      h0 (varraylist pred1 pred2 pred3 r (US.v hd1) (US.v hd2) (US.v hd3)) ==
-      h1 (varraylist pred1 pred2 pred3 r (US.v hd1) (US.v hd2) (US.v hd3)) /\
+      gs1 == gs0 /\
       // Functional property
-      pred2 (get_data (Seq.index (h1 (varraylist pred1 pred2 pred3 r (US.v hd1) (US.v hd2) (US.v hd3))) (US.v hd2)))
+      pred2 (get_data (Seq.index gs1 (US.v hd2)))
     )
 
-/// The order of the three lists does not matter, we can permute them in the varraylist predicate.
+/// The order of the four lists does not matter, we can permute them in the varraylist predicate.
 /// We permute here the first and second lists
 val permute12 (#a:Type) (#opened:inames)
-  (pred1 pred2 pred3: a -> prop)
+  (pred1 pred2 pred3 pred4: a -> prop)
   (r:A.array (cell a))
-  (hd1:nat)
-  (hd2:nat)
-  (hd3:nat) :
+  (hd1 hd2 hd3 hd4:nat) :
   SteelGhost unit opened
-    (varraylist pred1 pred2 pred3 r hd1 hd2 hd3)
-    (fun _ -> varraylist pred2 pred1 pred3 r hd2 hd1 hd3)
+    (varraylist pred1 pred2 pred3 pred4 r hd1 hd2 hd3 hd4)
+    (fun _ -> varraylist pred2 pred1 pred3 pred4 r hd2 hd1 hd3 hd4)
     (requires fun _ -> True)
     (ensures fun h0 _ h1 ->
+      let gs0 = h0 (varraylist pred1 pred2 pred3 pred4 r
+        hd1 hd2 hd3 hd4) in
+      let gs1 = h1 (varraylist pred2 pred1 pred3 pred4 r
+        hd2 hd1 hd3 hd4) in
       // Framing
-      h0 (varraylist pred1 pred2 pred3 r hd1 hd2 hd3) ==
-      h1 (varraylist pred2 pred1 pred3 r hd2 hd1 hd3)
+      gs1 == gs0
     )
 
-/// The order of the three lists does not matter, we can permute them in the varraylist predicate
+/// The order of the four lists does not matter, we can permute them in the varraylist predicate
 /// We permute here the first and third lists
 val permute13 (#a:Type) (#opened:inames)
-  (pred1 pred2 pred3: a -> prop)
+  (pred1 pred2 pred3 pred4: a -> prop)
   (r:A.array (cell a))
-  (hd1:nat)
-  (hd2:nat)
-  (hd3:nat) :
+  (hd1 hd2 hd3 hd4:nat) :
   SteelGhost unit opened
-    (varraylist pred1 pred2 pred3 r hd1 hd2 hd3)
-    (fun _ -> varraylist pred3 pred2 pred1 r hd3 hd2 hd1)
+    (varraylist pred1 pred2 pred3 pred4 r hd1 hd2 hd3 hd4)
+    (fun _ -> varraylist pred3 pred2 pred1 pred4 r hd3 hd2 hd1 hd4)
     (requires fun _ -> True)
     (ensures fun h0 _ h1 ->
+      let gs0 = h0 (varraylist pred1 pred2 pred3 pred4 r
+        hd1 hd2 hd3 hd4) in
+      let gs1 = h1 (varraylist pred3 pred2 pred1 pred4 r
+        hd3 hd2 hd1 hd4) in
       // Framing
-      h0 (varraylist pred1 pred2 pred3 r hd1 hd2 hd3) ==
-      h1 (varraylist pred3 pred2 pred1 r hd3 hd2 hd1)
+      gs1 == gs0
     )
 
-/// The order of the three lists does not matter, we can permute them in the varraylist predicate
-/// We permute here the second and third lists
-val permute23 (#a:Type) (#opened:inames)
-  (pred1 pred2 pred3: a -> prop)
+/// The order of the four lists does not matter, we can permute them in the varraylist predicate
+/// We permute here the first and third lists
+val permute14 (#a:Type) (#opened:inames)
+  (pred1 pred2 pred3 pred4: a -> prop)
   (r:A.array (cell a))
-  (hd1:nat)
-  (hd2:nat)
-  (hd3:nat) :
+  (hd1 hd2 hd3 hd4:nat) :
   SteelGhost unit opened
-    (varraylist pred1 pred2 pred3 r hd1 hd2 hd3)
-    (fun _ -> varraylist pred1 pred3 pred2 r hd1 hd3 hd2)
+    (varraylist pred1 pred2 pred3 pred4 r hd1 hd2 hd3 hd4)
+    (fun _ -> varraylist pred4 pred2 pred3 pred1 r hd4 hd2 hd3 hd1)
     (requires fun _ -> True)
     (ensures fun h0 _ h1 ->
+      let gs0 = h0 (varraylist pred1 pred2 pred3 pred4 r
+        hd1 hd2 hd3 hd4) in
+      let gs1 = h1 (varraylist pred4 pred2 pred3 pred1 r
+        hd4 hd2 hd3 hd1) in
       // Framing
-      h0 (varraylist pred1 pred2 pred3 r hd1 hd2 hd3) ==
-      h1 (varraylist pred1 pred3 pred2 r hd1 hd3 hd2)
+      gs1 == gs0
     )
 
 /// Reads at index [idx] in the array.
 inline_for_extraction noextract
 val read_in_place (#a:Type)
-  (#pred1 #pred2 #pred3: a -> prop)
+  (#pred1 #pred2 #pred3 #pred4: a -> prop)
   (r:A.array (cell a))
-  (hd1 hd2 hd3:Ghost.erased nat)
+  (hd1 hd2 hd3 hd4:Ghost.erased nat)
   (idx:US.t{US.v idx < A.length r})
   : Steel a
-          (varraylist pred1 pred2 pred3 r hd1 hd2 hd3)
-          (fun _ -> varraylist pred1 pred2 pred3 r hd1 hd2 hd3)
-          (requires fun _ -> True)
-          (ensures fun h0 res h1 ->
-            // Fucntional correctness
-            res == get_data (Seq.index (h0 (varraylist pred1 pred2 pred3 r hd1 hd2 hd3)) (US.v idx)) /\
-            // Framing
-            h0 (varraylist pred1 pred2 pred3 r hd1 hd2 hd3) ==
-            h1 (varraylist pred1 pred2 pred3 r hd1 hd2 hd3))
+  (varraylist pred1 pred2 pred3 pred4 r hd1 hd2 hd3 hd4)
+  (fun _ -> varraylist pred1 pred2 pred3 pred4 r hd1 hd2 hd3 hd4)
+  (requires fun _ -> True)
+  (ensures fun h0 res h1 ->
+    let gs0 = h0 (varraylist pred1 pred2 pred3 pred4 r
+      hd1 hd2 hd3 hd4) in
+    let gs1 = h1 (varraylist pred1 pred2 pred3 pred4 r
+      hd1 hd2 hd3 hd4) in
+    // Framing
+    gs1 == gs0 /\
+    // Functional correctness
+    res == get_data (Seq.index gs0 (US.v idx))
+  )
 
+//TODO: to be removed
 /// Updates the `data` field of the cell at index [idx] in the array [r] with [v]
-/// We define three different functions, depending on which list the element
-/// belongs to. In all three cases, we require [v] to satisfy the predicate
+/// We define four different functions, depending on which list the element
+/// belongs to. In all four cases, we require [v] to satisfy the predicate
 /// corresponding to a given list
 /// Note, we only expose the version for [hd1] to avoid duplication,
 /// but we can easily obtain versions for [hd2] and [hd3] using the
 /// permutations above. See instantiations in `src/ArrayList.fst`
 inline_for_extraction noextract
 val write_in_place (#a:Type)
-  (#pred1 #pred2 #pred3: a -> prop)
+  (#pred1 #pred2 #pred3 #pred4: a -> prop)
   (r:A.array (cell a))
-  (hd1 hd2 hd3:Ghost.erased nat)
+  (hd1 hd2 hd3 hd4:Ghost.erased nat)
   (idx:US.t{US.v idx < A.length r})
   (v:a)
-   : Steel unit
-          (varraylist pred1 pred2 pred3 r hd1 hd2 hd3)
-          (fun _ -> varraylist pred1 pred2 pred3 r hd1 hd2 hd3)
-          (requires fun h -> pred1 v /\ mem (US.v idx) hd1 (h (varraylist pred1 pred2 pred3 r hd1 hd2 hd3)))
-          (ensures fun h0 _ h1 -> True) // TODO
+  : Steel unit
+  (varraylist pred1 pred2 pred3 pred4 r hd1 hd2 hd3 hd4)
+  (fun _ -> varraylist pred1 pred2 pred3 pred4 r hd1 hd2 hd3 hd4)
+  (requires fun h0 ->
+    let gs0 = h0 (varraylist pred1 pred2 pred3 pred4 r hd1 hd2 hd3 hd4) in
+    pred1 v /\ mem (US.v idx) hd1 gs0
+  )
+  (ensures fun h0 _ h1 -> True)
 
 /// Removes the element at offset [idx] from the dlist pointed to by [hd1]
 /// Note, we only expose the version for [hd1] to avoid duplication,
@@ -337,25 +385,29 @@ val write_in_place (#a:Type)
 /// permutations above. See instantiations in `src/ArrayList.fst`
 inline_for_extraction noextract
 val remove (#a:Type)
-  (#pred1 #pred2 #pred3: a -> prop)
+  (#pred1 #pred2 #pred3 #pred4: a -> prop)
   (r:A.array (cell a))
   (hd1:US.t)
-  (hd2 hd3:Ghost.erased nat)
+  (hd2 hd3 hd4:Ghost.erased nat)
   (idx:US.t{US.v idx < A.length r})
-   : Steel US.t
-          (varraylist pred1 pred2 pred3 r (US.v hd1) hd2 hd3)
-          (fun hd' -> varraylist pred1 pred2 pred3 r (US.v hd') hd2 hd3)
-          (requires fun h -> mem (US.v idx) (US.v hd1) (h (varraylist pred1 pred2 pred3 r (US.v hd1) hd2 hd3)))
-          (ensures fun h0 hd' h1 ->
-            let gs0 = h0 (varraylist pred1 pred2 pred3 r (US.v hd1) hd2 hd3) in
-            let gs1 = h1 (varraylist pred1 pred2 pred3 r (US.v hd') hd2 hd3) in
-            ptrs_in (US.v hd') gs1 ==
-            FS.remove (US.v idx) (ptrs_in (US.v hd1) gs0) /\
-            ptrs_in hd2 gs1 == ptrs_in hd2 gs0 /\
-            ptrs_in hd3 gs1 == ptrs_in hd3 gs0 /\
-            (~ (mem_all (US.v idx) (US.v hd') hd2 hd3 gs1)) /\
-            dataify gs1 == dataify gs0
-          )
+  : Steel US.t
+  (varraylist pred1 pred2 pred3 pred4 r (US.v hd1) hd2 hd3 hd4)
+  (fun hd' -> varraylist pred1 pred2 pred3 pred4 r (US.v hd') hd2 hd3 hd4)
+  (requires fun h0 ->
+    let gs0 = h0 (varraylist pred1 pred2 pred3 pred4 r (US.v hd1) hd2 hd3 hd4) in
+    mem (US.v idx) (US.v hd1) gs0
+  )
+  (ensures fun h0 hd' h1 ->
+    let gs0 = h0 (varraylist pred1 pred2 pred3 pred4 r (US.v hd1) hd2 hd3 hd4) in
+    let gs1 = h1 (varraylist pred1 pred2 pred3 pred4 r (US.v hd') hd2 hd3 hd4) in
+    ptrs_in (US.v hd') gs1 ==
+    FS.remove (US.v idx) (ptrs_in (US.v hd1) gs0) /\
+    ptrs_in hd2 gs1 == ptrs_in hd2 gs0 /\
+    ptrs_in hd3 gs1 == ptrs_in hd3 gs0 /\
+    ptrs_in hd4 gs1 == ptrs_in hd4 gs0 /\
+    (~ (mem_all (US.v idx) (US.v hd') hd2 hd3 hd4 gs1)) /\
+    dataify gs1 == dataify gs0
+  )
 
 /// Requires that the element at offset [idx] does not belong to any dlist.
 /// If so, insert it at the head of list [hd1].
@@ -364,50 +416,54 @@ val remove (#a:Type)
 /// permutations above. See instantiations in `src/ArrayList.fst`
 inline_for_extraction noextract
 val insert (#a:Type)
-  (#pred1 #pred2 #pred3: a -> prop)
+  (#pred1 #pred2 #pred3 #pred4: a -> prop)
   (r:A.array (cell a))
-  (hd:US.t)
-  (hd2 hd3:Ghost.erased nat)
+  (hd1:US.t)
+  (hd2 hd3 hd4:Ghost.erased nat)
   (idx:US.t{idx <> null_ptr /\ US.v idx < A.length r})
   (v: a)
-   : Steel unit
-          (varraylist pred1 pred2 pred3 r (US.v hd) hd2 hd3)
-          (fun _ -> varraylist pred1 pred2 pred3 r (US.v idx) hd2 hd3)
-          (requires fun h -> pred1 v /\
-            (~ (mem_all (US.v idx) (US.v hd) hd2 hd3 (h (varraylist pred1 pred2 pred3 r (US.v hd) hd2 hd3)))))
-          (ensures fun h0 hd' h1 ->
-            let gs0 = h0 (varraylist pred1 pred2 pred3 r (US.v hd) hd2 hd3) in
-            let gs1 = h1 (varraylist pred1 pred2 pred3 r (US.v idx) hd2 hd3) in
-            ptrs_in (US.v idx) gs1 ==
-            FS.insert (US.v idx) (ptrs_in (US.v hd) gs0) /\
-            ptrs_in hd2 gs1 == ptrs_in hd2 gs0 /\
-            ptrs_in hd3 gs1 == ptrs_in hd3 gs0 /\
-            dataify gs1 == Seq.upd (dataify gs0) (US.v idx) v
-          )
+  : Steel unit
+  (varraylist pred1 pred2 pred3 pred4 r (US.v hd1) hd2 hd3 hd4)
+  (fun _ -> varraylist pred1 pred2 pred3 pred4 r (US.v idx) hd2 hd3 hd4)
+  (requires fun h0 ->
+    let gs0 = h0 (varraylist pred1 pred2 pred3 pred4 r (US.v hd1) hd2 hd3 hd4) in
+    pred1 v /\ (~ (mem_all (US.v idx) (US.v hd1) hd2 hd3 hd4 gs0))
+  )
+  (ensures fun h0 hd' h1 ->
+    let gs0 = h0 (varraylist pred1 pred2 pred3 pred4 r (US.v hd1) hd2 hd3 hd4) in
+    let gs1 = h1 (varraylist pred1 pred2 pred3 pred4 r (US.v idx) hd2 hd3 hd4) in
+    ptrs_in (US.v idx) gs1 ==
+    FS.insert (US.v idx) (ptrs_in (US.v hd1) gs0) /\
+    ptrs_in hd2 gs1 == ptrs_in hd2 gs0 /\
+    ptrs_in hd3 gs1 == ptrs_in hd3 gs0 /\
+    ptrs_in hd4 gs1 == ptrs_in hd4 gs0 /\
+    dataify gs1 == Seq.upd (dataify gs0) (US.v idx) v
+  )
 
 /// If the doubly linked lists fit in the first [k] elements of the array, then
 /// they also fit in the [k] + 1 first elements of the array, and we inserted
 /// element [k] in the first list
 inline_for_extraction noextract
 val extend (#a:Type)
-  (#pred1 #pred2 #pred3: a -> prop)
+  (#pred1 #pred2 #pred3 #pred4: a -> prop)
   (r:A.array (cell a))
   (hd:US.t{hd == null_ptr \/ US.v hd < A.length r})
-  (hd2 hd3:Ghost.erased nat)
+  (hd2 hd3 hd4:Ghost.erased nat)
   (k:US.t{US.v k + 1 <= A.length r /\ US.fits (US.v k + 1)})
   (v:a)
   : Steel unit
-          (varraylist pred1 pred2 pred3 (A.split_l r k) (US.v hd) hd2 hd3 `star`
-            A.varray (A.split_l (A.split_r r k) 1sz))
-          (fun _ -> varraylist pred1 pred2 pred3 (A.split_l r (k `US.add` 1sz)) (US.v k) hd2 hd3)
-          (requires fun _ ->
-            k <> null_ptr /\ pred1 v)
-          (ensures fun h0 _ h1 ->
-            let gs0 = h0 (varraylist pred1 pred2 pred3 (A.split_l r k) (US.v hd) hd2 hd3) in
-            let gs1 = h1 (varraylist pred1 pred2 pred3 (A.split_l r (k `US.add` 1sz)) (US.v k) hd2 hd3) in
-            ptrs_in (US.v k) gs1 ==
-            FS.insert (US.v k) (ptrs_in (US.v hd) gs0) /\
-            ptrs_in hd2 gs1 == ptrs_in hd2 gs0 /\
-            ptrs_in hd3 gs1 == ptrs_in hd3 gs0 /\
-            dataify gs1 == Seq.append (dataify gs0) (Seq.create 1 v)
-          )
+  (varraylist pred1 pred2 pred3 pred4 (A.split_l r k) (US.v hd) hd2 hd3 hd4 `star`
+    A.varray (A.split_l (A.split_r r k) 1sz))
+  (fun _ -> varraylist pred1 pred2 pred3 pred4 (A.split_l r (k `US.add` 1sz)) (US.v k) hd2 hd3 hd4)
+  (requires fun _ ->
+    k <> null_ptr /\ pred1 v)
+  (ensures fun h0 _ h1 ->
+    let gs0 = h0 (varraylist pred1 pred2 pred3 pred4 (A.split_l r k) (US.v hd) hd2 hd3 hd4) in
+    let gs1 = h1 (varraylist pred1 pred2 pred3 pred4 (A.split_l r (k `US.add` 1sz)) (US.v k) hd2 hd3 hd4) in
+    ptrs_in (US.v k) gs1 ==
+    FS.insert (US.v k) (ptrs_in (US.v hd) gs0) /\
+    ptrs_in hd2 gs1 == ptrs_in hd2 gs0 /\
+    ptrs_in hd3 gs1 == ptrs_in hd3 gs0 /\
+    ptrs_in hd4 gs1 == ptrs_in hd4 gs0 /\
+    dataify gs1 == Seq.append (dataify gs0) (Seq.create 1 v)
+  )
